
$$\begin{cases}
x'=x^2-y^2-1 \\
y'=-2y
\end{cases}$$



$$\begin{cases}
x'=-6x+2xy \\
y'=y^2-x^2
\end{cases}$$

Sustituimos $x'=0$ y $y'=0$.
$$\begin{cases}
-6x+2xy=0 \\
y^2-x^2=0
\end{cases}$$De (1), $$-2x(3-y)=0$$
$$\implies x=0, \implies y=3$$
Sustituyendo en (2), $$\text{Si x=0,}\quad y^2-x^2=0\implies y^2=0\implies y=0$$
$$\text{Si y=3}\quad y^2-x^2=0\implies 9-x^2=0\implies x=\pm 3$$
$$\therefore P_{2}(3,3)\text{ y }P_{3}(-3,3)$$

$$J=\begin{pmatrix}-6+2y & 2x \\
-2x & 2y\end{pmatrix}$$
Para $P_{1}(0,0)$, $$A=\begin{pmatrix}-6 & 0 \\
0 & 0\end{pmatrix}$$

#TODO tome fotos
